# regression

## bivariate data

Data obtained when observing two characteristics of one object

$$
(x_1, y_1), (x_2, y_2), \cdots, (x_n, y_n)
$$

## Sample covariance

Linear relationship

$$
s_{xy} = \frac{1}{n-1}\sum_{i=1}^n(x_i - \bar x)(y_i - \bar y) = \frac{1}{n-1}(\sum_{i=1}^nx_iy_i - n\bar x\bar y)
$$

## Sample correlation

$$
r_{xy} = \frac{s_{xy}}{s_xs_y}
$$

Note that $-1 \le r_{xy} \le 1$

## Spearman correlation coefficient

Measure of monotonicity

$$
\rho_{xy} = \frac{s_{r(x)r(y)}}{s_{r(x)}s_{r(y)}}
$$

Where $r(x)$ denotes the rank of $x$

If there are no ties:

$$
\rho_{xy} = 1 - \frac{6\sum_{i=1}^n d_i^2}{n(n^2 - 1)}
$$

Where $d_i = r(x_i) - r(y_i)$

## relationships

### deterministic

$y = f(x)$

### nondeterministic

$y = f(x) + \varepsilon$

## linear regression

$$
Y_i = \beta_0 + \beta_1x_i + \varepsilon_i
$$

- $\varepsilon_1, \cdots, \varepsilon_n \sim N(0, \sigma^2)$
- $\beta_0$ is called the intercept
- $\beta_1$ is called the slope

Regression line $\hat y = \hat \beta_0 + \hat \beta_1 x$ can be estimated using least squares. These estimators are:

- $\hat \beta_1 = \frac{s_{xy}}{s_x^2}$
- $\hat \beta_0 = \bar y - \hat \beta_1 \bar x$

Unbiased estimator for $\sigma^2$: $s_R^2 = \frac{1}{n-2} \sum_{i=1}^n(y_i - \hat y_i)^2$

### parameters

$$
\hat \beta_0 \sim N(\beta_0, \sqrt{\sigma^2(\frac{1}{n} + \frac{\bar x^2}{(n-1)s_X^2})})
$$

$$
\frac{\hat \beta_0 - \beta_0}{\sqrt{s_R^2(\frac{1}{n} + \frac{\bar x^2}{(n-1)s_X^2})}} \sim t_{n-2}
$$

$$
\hat \beta_1 \sim N(\beta_1, \sqrt{\frac{\sigma^2}{(n-1)s_X^2}})
$$

$$
\frac{\hat \beta_1 - \beta_1}{\sqrt{\frac{s_R^2}{(n-1)s_X^2}}} \sim t_{n-2}
$$

## coefficient of determination

Goodness of fit

$$
R^2 = r^2_{(x,y)}
$$

is the percentage of the sample variability in the $y$ variable is explained by the model (linear dependence on $x$). Higher the better.

### variability decomposition

$$
\begin{aligned}
	\text{Total sum of squares (SST)} &= \text{Residual sum of squares (SSR)} &&+ \text{Model sum of squares (SSM)} \\
	\sum_i (y_i - \bar y)^2 &= \sum_i (y_i - \hat y)^2 &&+ \sum_i (\hat y - \bar y)^2 \\
\end{aligned}
$$

then

$$
R^2 = 1 - \frac{\text{SSR}}{\text{SST}} = \frac{\text{SSM}}{\text{SST}}
$$
